new/trusted_code/sync/atomic.v
@@ -13,5 +13,10 @@ Definition StoreUint64 : val :=
 Definition AddUint64 : val :=
   λ: "addr", #() #().
 
+Definition CompareAndSwapUint64 : val :=
+  λ: "addr" "old" "new",
+    Snd (CmpXchg "addr" "old" "new")
+.
+
 End code.
 End atomic.
